concur/StackingRefine.v
@@ -1,0 +1,207 @@
+Require Import LanguageInterface CallconvAlgebra Invariant.
+Require Import CKLR Inject InjectFootprint Extends.
+Require Import Linear Mach Locations Conventions.
+Require Import ValueAnalysis.
+Require Import Allocproof Lineartyping Asmgenproof0.
+Require Import Maps Stacklayout.
+
+Require Import CallconvBig CallConvAlgebra InjpAccoComp VCompBig.
+Require Import Separation StackingproofC CallConv CallConvLibs.
+Import GS.
+
+Local Open Scope sep_scope.
+
+Record cc_stacking_world_injp :=
+  stkjw {
+    stk_w : injp_world;
+    stk_sg : signature;
+    stk_ls1 : Locmap.t;
+    stk_rs2 : regset;
+    stk_sp2 : val;
+    stk_m2 : mem;
+    }.
+
+Definition stacking_get_injp (ws: cc_stacking_world_injp) := stk_w ws.
+
+Definition stacking_set_injp (ws: cc_stacking_world_injp) (w : injp_world) :=
+  match ws with stkjw w' sg ls1 rs2 sp2 m2 => stkjw w sg ls1 rs2 sp2 m2 end.
+
+Program Instance lens_stacking_injp : Lens (cc_stacking_world_injp) injp_world :=
+  {
+    get := stacking_get_injp;
+    set := stacking_set_injp;
+  }.
+Next Obligation. destruct t. reflexivity. Qed.
+Next Obligation. destruct t. reflexivity. Qed.
+Next Obligation. destruct t. reflexivity. Qed.
+
+Program Instance STKworld : World (cc_stacking_world_injp) :=
+  {
+    w_state := injp_world;
+    w_lens := lens_stacking_injp;
+    w_acci := injp_acci;
+    w_acce := injp_acce;
+    w_acci_trans := injp_acci_preo;
+  }.
+
+Inductive pointer_tid (tid : nat) : val -> Prop :=
+|pointer_tid_intro b ofs:
+  fst b = tid -> pointer_tid tid (Vptr b ofs).
+                                          
+Inductive cc_stacking_injp_mq: (cc_stacking_world_injp) -> _ -> _ -> Prop :=
+| cc_stacking_mq_intro vf1 vf2 sg ls1 m1 sp2 ra2 rs2 m2 f
+    (SPL: pointer_tid (Mem.tid (Mem.support m1)) sp2)
+    (RA: ra2 <> Vundef)
+    (Hm: Mem.inject f m1 m2):
+  vf1 <> Vundef -> Val.inject f vf1 vf2 ->
+  (forall r, Val.inject f (ls1 (Locations.R r)) (rs2 r)) ->
+  m2 |= contains_init_args sg f ls1 m2 sp2 ->
+  (forall b ofs, loc_init_args (size_arguments sg) sp2 b ofs ->
+            loc_out_of_reach f m1 b ofs) ->
+  Val.has_type sp2 Tptr ->
+  Val.has_type ra2 Tptr ->
+  cc_stacking_injp_mq
+    (stkjw (injpw f m1 m2 Hm) sg ls1 rs2 sp2 m2)
+    (lq vf1 sg ls1 m1)
+    (mq vf2 sp2 ra2 rs2 m2).
+
+Inductive cc_stacking_injp_mr : (cc_stacking_world_injp) -> _ -> _ -> Prop :=
+| cc_stacking_mr_intro sg ls1 ls1' m1' sp2 m2 rs2 rs2' m2' f'
+    (Hm' : Mem.inject f' m1' m2'):
+    (forall r,
+      In r (regs_of_rpair (loc_result sg)) ->
+      Val.inject f' (ls1' (Locations.R r)) (rs2' r)) ->
+    (forall r,
+        is_callee_save r = true -> rs2 r = rs2' r) ->
+        
+      (* Val.inject f' (ls1 (Locations.R r)) (rs2' r)) -> *)
+    Mem.unchanged_on (loc_init_args (size_arguments sg) sp2) m2 m2' ->
+    (forall b ofs, loc_init_args (size_arguments sg) sp2 b ofs ->
+                   loc_out_of_reach f' m1' b ofs) ->
+    cc_stacking_injp_mr
+      (stkjw (injpw f' m1' m2' Hm') sg ls1 rs2 sp2 m2)
+      (lr ls1' m1')
+      (mr rs2' m2').
+
+Program Definition cc_stacking_injp : GS.callconv li_locset li_mach := {|
+    GS.ccworld := cc_stacking_world_injp;
+    GS.ccworld_world := STKworld;
+    GS.match_senv w := CKLR.match_stbls injp (stacking_get_injp w);
+    GS.match_query := cc_stacking_injp_mq;
+    GS.match_reply := cc_stacking_injp_mr
+                                                                      |}.
+Next Obligation.
+  inv H. inv H1. eauto.
+Qed.
+Next Obligation.
+  inv H.
+  eapply Genv.valid_for_match in H2.
+  apply H2. eauto.
+Qed.
+
+Lemma cctrans_locset_injp_stacking : cctrans (locset_injp @ cc_stacking_injp) cc_stacking_injp.
+Proof.
+  constructor.
+  econstructor. instantiate (1:= match_12_cctrans).
+  - red. intros [w sg ls1 rs3 sp3 m3] se1 se2 q1 q2 Hse Hq.
+    inv Hse. simpl in H2. inv Hq. inv H3. clear Hm Hm0.
+    (* Compute  ccworld (locset_injp @ cc_stacking_injp). *)
+    exists (se1, (sg, injpw (meminj_dom f) m1 m1 (mem_inject_dom f m1 m2 Hm1), (stkjw(injpw f m1 m2 Hm1) sg ls1 rs3 sp3 m2))).
+    repeat apply conj.
+    + simpl. split. econstructor; eauto. eapply match_stbls_dom; eauto.
+      econstructor; eauto.
+    + simpl. exists (lq vf1 sg ls1 m1). split. econstructor; simpl; eauto.
+      eapply val_inject_dom; eauto. red. intros.
+      inv H2.
+      eapply val_inject_dom; eauto. destruct H14 as [A [B C]].
+      exploit C; eauto. intros [v' [D E]].
+      eapply val_inject_dom; eauto.
+      econstructor; eauto.
+    + simpl. constructor; eauto. rewrite meminj_dom_compose. reflexivity.
+    + simpl. econstructor; eauto. intros. unfold meminj_dom in H3.
+      destruct (f b1) as [[? ?]|] eqn: Hf; inv H3. congruence.
+      intros. exists b2, ofs2. split. auto. unfold meminj_dom. rewrite H4.
+      replace (ofs2 - ofs2) with 0 by lia. reflexivity.
+    + simpl. intros r1 r3 wp1 wp2 wp1' Hmatch [Hae1 Hae2] [Hai1 Hai2] Hr.
+      simpl in Hae1, Hae2. destruct wp1' as [wp11' wp12'].
+      destruct wp1 as [wp11 wp12]. simpl in *.
+      destruct wp11' as [j12 m1' m2' Hm1'].
+      destruct wp12' as [j23 m2'_ m3' Hm2'].
+      destruct Hr as [r' [Hr1 Hr2]]. inv Hr1. inv Hr2. inv H3. clear Hm'0 Hm'2 Hm'1.
+      clear Hm0 Hm2 Hm3. rename m1'0 into m1'. rename m2'0 into m2'.
+      exists (injpw (compose_meminj j12 j23) m1' m3' (Mem.inject_compose _ _ _ _ _ Hm1' Hm2')).
+      repeat apply conj; eauto.
+      -- eapply injp_comp_acce. 3: apply Hae1. 3: apply Hae2.
+         econstructor; eauto.
+         econstructor; eauto.
+      -- inv Hmatch. eapply injp_comp_acci; eauto. econstructor; eauto.
+      -- econstructor; eauto. intros.
+         eapply val_inject_compose; eauto.
+         intros.  red. intros.
+         specialize (H25 _ _ H3). red in H25.
+         unfold compose_meminj in H4. repeat destr_in H4.
+         intro. exploit H25; eauto.
+         replace (ofs - z0) with (ofs - (z + z0) + z) by lia.
+         eapply Mem.perm_inject; eauto.
+  - red. intros wp1 wp2 w1 se1 se2 q1 q3 Hs Hq HACI Hmatch.
+    inv Hmatch. destruct w1 as [x [[sg' w11] [w12 sg ls2 rs3 sp3 m3]]].
+    inv HACI. simpl in H1,H2. simpl in wp1, wp2.
+    (** Basiclly the same as old injp_comp (the hard part), plus a ACCI preservation *)
+    destruct w11 as [j12' m1' m2' Hm12'].
+    destruct w12 as [j23' m2'_ m3' Hm23'].
+    destruct Hs as [Hs1 Hs2]. inv Hs1. inv Hs2.
+    destruct Hq as [q2 [Hq1 Hq2]]. inv Hq1. inv Hq2. inv H5. simpl in H4. rename ls0 into ls2.
+    rename m1 into m1'. rename m2 into m2'. rename m3 into m3'.
+    exists (stkjw (injpw (compose_meminj j12' j23')  m1' m3' (Mem.inject_compose _ _ _ _ _ Hm12' Hm23')) sg' ls1 rs3 sp3 m3' ).
+    repeat apply conj; eauto.
+    + simpl. inv H; simpl in *.
+      eapply injp_comp_acci; eauto.
+      econstructor; eauto.
+      econstructor; eauto.
+    + econstructor; eauto.
+      eapply Genv.match_stbls_compose; eauto.
+    + simpl.
+      econstructor; simpl; eauto. inv SPL. constructor.
+      erewrite inject_tid; eauto.
+      eapply val_inject_compose; eauto.
+      intros. eapply val_inject_compose; eauto. eapply H4; eauto. constructor.
+      destruct H29 as [A [B C]]. split. auto. split. auto. intros.
+      exploit C; eauto. intros [v [Hl Hinj]].  exists v.
+      split. eauto. eapply val_inject_compose. eapply H4; eauto. constructor. eauto.
+      eauto.
+      intros.  red. intros.
+      specialize (H30 _ _ H5). red in H30.
+      unfold compose_meminj in H11. repeat destr_in H11.
+      intro. exploit H30; eauto.
+      replace (ofs - z0) with (ofs - (z + z0) + z) by lia.
+      eapply Mem.perm_inject; eauto.
+    + (** The accessbility construction : use acco*)
+      intros r1 r3 wp2' ACCO1 MR. simpl in ACCO1. simpl in MR.
+      destruct wp2' as [j13'' m1'' m3'' Hm13']. inv MR.
+      simpl in H3, H4. 
+      assert (Hhidden: external_mid_hidden (injpw j12' m1' m2' Hm12') (injpw j23' m2' m3' Hm23')).
+      destruct wp1 as [w w0]. destruct w, w0.  inv H0.
+      exploit external_mid_hidden_acci; eauto. econstructor; eauto.
+      exploit injp_acce_outgoing_constr; eauto.
+      intros (j12'' & j23'' & m2'' & Hm12'' & Hm23'' & COMPOSE & ACCE1 & ACCE2 & HIDDEN & OUT).
+      exists ((injpw j12'' m1'' m2'' Hm12''),(injpw j23'' m2'' m3'' Hm23'')).
+      repeat apply conj; eauto.
+      -- simpl.
+         generalize (loc_result_always_one sg'). intro Hresult.
+         destruct Hresult as [r Hresult]. rewrite Hresult in *.
+         exploit H22; eauto. simpl. left. reflexivity. intro Hinjresult.
+         exploit compose_meminj_midvalue. rewrite COMPOSE in Hinjresult. eauto.
+         intros [vres2 [RES1 RES2]]. 
+         set (ls2' l := if Loc.eq l (R r) then vres2 else ls1' l).
+         exists (lr ls2' m2''). split. econstructor; eauto. simpl.
+         red. intros. rewrite Hresult in H5.  inv H5. simpl.
+         unfold ls2'.
+         rewrite pred_dec_true. eauto. reflexivity. inv H11.
+         constructor.
+         econstructor; eauto. intros. rewrite Hresult in H5. inv H5.
+         unfold ls2'.
+         rewrite pred_dec_true. eauto. reflexivity. inv H11.
+      -- simpl. econstructor; eauto.
+Qed.
+        
+      
